Prove Interpreter enforcement through predicate of synchronization

src/Refine.v
@@ -1,5 +1,12 @@
 Require Import FreeSpec.Program.
 Require Import FreeSpec.Interp.
+Require Import FreeSpec.Contract.
+Require Import FreeSpec.Abstract.
+
+(** * Stateful Refinement
+
+    ** Definition
+ *)
 
 Definition StatefulRefinement
            (Ii: Type -> Type)
@@ -23,6 +30,131 @@ Definition StatefulInterpret
                   (snd (evalProgram (snd st) (sr A i (fst st))),
                    (execProgram (snd st) (sr A i (fst st))))))
              (s, int).
+
+(** ** Contract Enforcement
+
+    We consider so-called “predicates of synchronization” between two
+    abstract States [Si] (input) and [So] (output) linked by a
+    concrete state [S].
+ *)
+
+Definition sync_pred
+           (Si So: Type)
+           (S: Type)
+  := Si -> S -> So -> Type.
+
+Definition compliant_refinement
+           {Si So: Type}
+           {Ii Io: Interface}
+           {S: Type}
+           (sr: StatefulRefinement Ii Io S)
+           (master: Contract Si Ii)
+           (slave: Contract So Io)
+           (sync: sync_pred Si So S) :=
+  forall (si: Si)
+         (s: S)
+         (so: So)
+         {A: Type}
+         (i: Ii A),
+    sync si s so
+    -> requirements master i si
+    -> contractfull_program slave so (sr A i s).
+
+Definition sync_preservation
+           {Si So: Type}
+           {Ii Io: Interface}
+           {S: Type}
+           (sr: StatefulRefinement Ii Io S)
+           (master: Contract Si Ii)
+           (slave: Contract So Io)
+           (sync: sync_pred Si So S) :=
+  forall (si: Si)
+         (s: S)
+         (so: So)
+         (int: Interp Io)
+         (Henf: Enforcer int slave so)
+         {A: Type}
+         (i: Ii A),
+  sync si s so
+  -> requirements master i si
+  -> sync (abstract_step master i (fst (evalProgram int (sr A i s))) si)
+          (snd (evalProgram int (sr A i s)))
+          (contract_derive (sr A i s) int slave so).
+
+Definition sync_promises
+           {Si So: Type}
+           {Ii Io: Interface}
+           {S: Type}
+           (sr: StatefulRefinement Ii Io S)
+           (master: Contract Si Ii)
+           (slave: Contract So Io)
+           (sync: sync_pred Si So S) :=
+  forall (si: Si)
+         (s: S)
+         (so: So)
+         (int: Interp Io)
+         (Henf: Enforcer int slave so)
+         {A: Type}
+         (i: Ii A),
+  sync si s so
+  -> requirements master i si
+  -> promises master i (fst (evalProgram int (sr A i s))) si.
+
+Theorem enforcer_refinement
+        {Si So: Type}
+        {Ii Io: Interface}
+        {S: Type}
+        (sr: StatefulRefinement Ii Io S)
+        (master: Contract Si Ii)
+        (slave: Contract So Io)
+        (sync: sync_pred Si So S)
+        (Hsyncpres: sync_preservation sr master slave sync)
+        (Hsyncp: sync_promises sr master slave sync)
+        (Hcompliant: compliant_refinement sr master slave sync)
+  : forall (si: Si)
+           (s: S)
+           (so: So)
+           (int: Interp Io)
+           (Henf: Enforcer int slave so),
+    sync si s so
+    -> Enforcer (StatefulInterpret sr s int) master si.
+Proof.
+  cofix.
+  intros si s so int Henf Hsync.
+  constructor.
+  + intros A i Hreq.
+    unfold sync_promises in Hsyncp.
+    assert (evalInstruction (StatefulInterpret sr s int) i = fst (evalProgram int (sr A i s)))
+      as Heq by reflexivity.
+    rewrite Heq.
+    apply (Hsyncp si s so int Henf A i Hsync Hreq).
+  + intros A i Hreq.
+    unfold compliant_refinement in Hcompliant.
+    assert (contractfull_program slave so (sr A i s))
+      as Hcp
+        by  apply (Hcompliant si s so A i Hsync Hreq).
+    assert (execInstruction (StatefulInterpret sr s int) i
+            = StatefulInterpret sr
+                                (snd (evalProgram int (sr A i s)))
+                                (execProgram int (sr A i s)))
+      as Hassoc
+        by reflexivity.
+    rewrite Hassoc.
+    apply (enforcer_refinement _ _ (contract_derive (sr A i s) int slave so)).
+    ++ rewrite <- (abstract_exec_exec_program_same (sr A i s)
+                                                   so
+                                                   (abstract_step slave)
+                                                   int).
+       apply (enforcer_contractfull_enforcer _ _ _ int Henf Hcp).
+    ++ apply Hsyncpres.
+       +++ exact Henf.
+       +++ exact Hsync.
+       +++ exact Hreq.
+Qed.
+
+(** * Pure Refinement
+
+ *)
 
 Definition PureRefinement
            (Ii: Type -> Type)
